@prefix rdf: <http://www.w3.org/1999/02/22-rdf-syntax-ns#> .
@prefix rdfs: <http://www.w3.org/2000/01/rdf-schema#> .
@prefix owl: <http://www.w3.org/2002/07/owl#> .
@prefix dcterms: <http://purl.org/dc/terms/> .
@prefix sioc: <http://rdfs.org/sioc/ns#> .

<http://rdfs.org/sioc/access#>
    dcterms:description "Extends the SIOC Core Ontology (Semantically-Interlinked Online Communities) by defining basic information on permissions and access rights." ;
    dcterms:title "SIOC Access Ontology Module" ;
    a owl:Ontology, owl:Thing ;
    rdfs:seeAlso <http://rdfs.org/sioc/spec/#sec-modules> ;
    owl:imports <http://rdfs.org/sioc/ns#> .

<http://rdfs.org/sioc/access#Permission>
    a rdfs:Class, owl:Class ;
    rdfs:comment "A Permission describes a type of action that can be performed on an object that is within the scope of a Role, e.g. a Site, Forum, etc."@en ;
    rdfs:isDefinedBy <http://rdfs.org/sioc/access#> ;
    rdfs:label "Permission"@en .

<http://rdfs.org/sioc/access#Status>
    a rdfs:Class, owl:Class ;
    rdfs:comment "A Status can be assign to content Item to indicate its publication status (e.g. public, draft, etc.). This class is used to define different types of status."@en ;
    rdfs:isDefinedBy <http://rdfs.org/sioc/access#> ;
    rdfs:label "Status"@en .

<http://rdfs.org/sioc/access#has_permission>
    a rdf:Property, owl:ObjectProperty ;
    rdfs:comment "A Permission assigned to a Role."@en ;
    rdfs:domain sioc:Role ;
    rdfs:isDefinedBy <http://rdfs.org/sioc/access#> ;
    rdfs:label "has permission"@en ;
    rdfs:range <http://rdfs.org/sioc/access#Permission> .

<http://rdfs.org/sioc/access#has_status>
    a rdf:Property, owl:ObjectProperty ;
    rdfs:comment "The Status of a content Item (e.g. public, draft)."@en ;
    rdfs:domain sioc:Item ;
    rdfs:isDefinedBy <http://rdfs.org/sioc/access#> ;
    rdfs:label "has status"@en ;
    rdfs:range <http://rdfs.org/sioc/access#Status> .

